Congruence_Closure_Explain/CC_Explain.thy
@@ -4,10 +4,166 @@ theory CC_Explain
 begin 
 
 
+
+section \<open>Explain definition\<close>
+
+text \<open>The highest node is in this case the same as the rep_of, because we do not 
+      have the optimisation of checking which equivalence class is bigger, 
+      we just make the union in the given order. When adding this optimisation,
+      a highest_node function must be also implemented. \<close>
+
+text \<open>There are three variables changed by the function \<open>explain_along_path\<close>: 
+
+      The overall output of explain
+      The Union Find list of the additional union find, which is local to the explain function
+      The list of pending proofs, which need to be recursively called with cc_explain
+      
+      These are the three values returned by this function.\<close>
+
+function (domintros) explain_along_path :: "congruence_closure \<Rightarrow> nat list \<Rightarrow> nat \<Rightarrow> nat \<Rightarrow> 
+    (equation set * nat list * (nat * nat) list)"
+  where 
+"explain_along_path cc l a c = 
+(if rep_of l a = rep_of l c 
+then
+  ({}, l, [])
+else
+  (let b = (proof_forest cc) ! rep_of l a in 
+    (
+    case the ((pf_labels cc) ! rep_of l a) of 
+        One a' \<Rightarrow>  
+          (let (output, new_l, pending) = explain_along_path cc (ufa_union l a b) b c
+          in ({a'} \<union> output, new_l, pending))
+        | Two (F a\<^sub>1 a\<^sub>2 \<approx> a') (F b\<^sub>1 b\<^sub>2 \<approx> b') \<Rightarrow> 
+          (let (output, new_l, pending) = explain_along_path cc (ufa_union l a b) b c
+          in ({(F a\<^sub>1 a\<^sub>2 \<approx> a'), (F b\<^sub>1 b\<^sub>2 \<approx> b')} \<union> output, new_l, [(a\<^sub>1, a\<^sub>2), (b\<^sub>1, b\<^sub>2)] @ pending))
+    )
+  )
+)"
+  by pat_completeness auto
+
+lemma explain_along_path_simp1:
+  assumes "rep_of l a = rep_of l c"
+  shows "explain_along_path cc l a c = ({}, l, [])"
+proof-
+  have "explain_along_path_dom (cc, l, a, c)"
+    using assms explain_along_path.domintros by blast
+  then show ?thesis using explain_along_path.psimps 
+    by (simp add: assms)
+qed
+
+lemma explain_along_path_simp2:
+  assumes "rep_of l a \<noteq> rep_of l c"
+"(pf_labels cc) ! rep_of l a = Some (One a')"
+"(output, new_l, pend) = explain_along_path cc (ufa_union l a ((proof_forest cc) ! rep_of l a)) 
+((proof_forest cc) ! rep_of l a) c"
+  shows "explain_along_path cc l a c = ({a'} \<union> output, new_l, pend)"
+proof-
+  have "explain_along_path_dom (cc, l, a, c)"
+    using assms explain_along_path.domintros sorry
+  then show ?thesis using explain_along_path.psimps unfolding Let_def
+    by (metis (no_types, lifting) assms case_prod_conv option.sel pending_equation.simps(5))
+qed
+
+lemma explain_along_path_simp3:
+  assumes "rep_of l a \<noteq> rep_of l c"
+"(pf_labels cc) ! rep_of l a = Some (Two (F a\<^sub>1 a\<^sub>2 \<approx> a') (F b\<^sub>1 b\<^sub>2 \<approx> b'))"
+"(output, new_l, pend) = explain_along_path cc (ufa_union l a ((proof_forest cc) ! rep_of l a)) 
+((proof_forest cc) ! rep_of l a) c"
+  shows "explain_along_path cc l a c = ({(F a\<^sub>1 a\<^sub>2 \<approx> a'), (F b\<^sub>1 b\<^sub>2 \<approx> b')} \<union> output, new_l, [(a\<^sub>1, a\<^sub>2), (b\<^sub>1, b\<^sub>2)] @ pend)"
+proof-
+  have "explain_along_path_dom (cc, l, a, c)"
+    using assms explain_along_path.domintros sorry
+  then show ?thesis using explain_along_path.psimps unfolding Let_def
+    using assms case_prod_conv option.sel pending_equation.simps(6) equation.simps(6) 
+    by (metis (no_types, lifting))
+qed
+
+function cc_explain :: "congruence_closure \<Rightarrow> nat list \<Rightarrow> (nat * nat) list \<Rightarrow> equation set"
+  where
+"cc_explain cc l [] = {}"
+| "cc_explain cc l ((a, b) # xs) =
+(if are_congruent cc (a \<approx> b)
+then
+  (let c = lowest_common_ancestor (proof_forest cc) a b;
+   (output1, new_l, pending1) = explain_along_path cc l a c;
+   (output2, new_new_l, pending2) = explain_along_path cc new_l b c
+  in
+    output1 \<union> output2 \<union> cc_explain cc new_new_l (xs @ pending1 @ pending2))
+else cc_explain cc l xs)
+"
+  by pat_completeness auto
+
+
+text "To show about pfl: left a = i and right a = pf ! i or opposite
+also it's never None if pf ! i ~= i."
+
+fun pending_set_explain :: "(nat * nat) list \<Rightarrow> equation set"
+  where
+"pending_set_explain pend = set (map (\<lambda>(a,b) . (a \<approx> b)) pend)"
+
+lemma explain_along_path_correctness:
+  assumes "ufa_invar pf"
+"a < length pf"
+"c < length pf"
+"path pf c pAC a"
+"length l = length pf"
+"explain_along_path \<lparr>cc_list = cc_l, use_list = u, lookup = t, pending = pe, 
+proof_forest = pf, pf_labels = pfl, input = ip\<rparr> l a c = (output, new_l, pend)"
+shows "(a \<approx> c) \<in> Congruence_Closure (representatives_set l \<union> output 
+\<union> pending_set_explain pend)"
+  using assms proof(induction arbitrary: "output" new_l pend l pAC rule: rep_of_induct)
+  case (base i)
+  then have "c = i" using path_root by auto
+  then show ?case by blast
+next
+  case (step i)
+  then show ?case proof(cases "rep_of l i = rep_of l c")
+    case True
+    then have "i \<approx> c \<in> Congruence_Closure (representatives_set l)"
+      using CC_same_rep_representatives_set[of l i c] step by argo
+    then show ?thesis 
+      using Congruence_Closure_split_rule by auto
+  next
+    case False
+    with step path_butlast have path_to_parent: "path pf c (butlast pAC) (pf ! i)" 
+      by blast
+    obtain output' new_l' pend' where recursive_step: "explain_along_path
+     \<lparr>cc_list = cc_l, use_list = u, lookup = t, pending = pe, proof_forest = pf, 
+pf_labels = pfl, input = ip\<rparr>
+     (ufa_union l i (pf ! i)) (pf ! i) c = (output', new_l', pend')"
+      using prod_cases3 by blast
+    with step path_to_parent recursive_step have "(pf ! i \<approx> c) \<in>
+ Congruence_Closure (representatives_set (ufa_union l i (pf ! i)) \<union> output' 
+\<union> pending_set_explain pend')" by simp
+    show ?thesis proof(cases "the (pfl ! rep_of l i)")
+      case (One a')
+      then have *: "pfl ! rep_of l i = Some (One a')" sorry
+(*TODO add pfl invar, similar to pending invar*)
+have dom: "explain_along_path_dom
+     (\<lparr>cc_list = cc_l, use_list = u, lookup = t, pending = pe, proof_forest = pf, pf_labels = pfl, input = ip\<rparr>, 
+l,i, c)" sorry 
+   have "(output, new_l, pend) = ({a'} \<union> output', new_l', pend')" 
+     using step(8) explain_along_path_simp2[OF False] One False * sledgehammer
+     by (auto split: pending_equation.splits prod.splits)
+      then show ?thesis sorry
+    next
+      case (Two x21 x22)
+      then show ?thesis sorry
+    qed
+  qed
+qed
+
 subsection \<open>Correctness of explain\<close>
 
-lemma "are_congruent cc (a \<approx> b) \<Longrightarrow> cc_invar cc \<Longrightarrow>
-  Congruence_Closure (cc_explain cc ([0..<nr_vars cc]) [(a, b)]) (a \<approx> b)"
+lemma cc_explain_correct:
+  assumes "are_congruent cc (a \<approx> b)" "cc_invar cc"
+  shows "(a \<approx> b) \<in> Congruence_Closure (cc_explain cc ([0..<nr_vars cc]) [(a, b)])"
+  sorry
+
+lemma cc_explain_valid:
+  assumes "are_congruent cc (a \<approx> b)" "cc_invar cc"
+  shows "cc_explain cc ([0..<nr_vars cc]) [(a, b)] \<subseteq> input cc"
   sorry
 
 end
